Rearranged some stuffs; to merge

src/Inline.v
@@ -5,14 +5,6 @@ Require Import Syntax Wf.
 Set Implicit Arguments.
 
 Section PhoasUT.
-  Definition typeUT (k: Kind): Type := unit.
-  Definition fullTypeUT := fullType typeUT.
-  Definition getUT (k: FullKind): fullTypeUT k :=
-    match k with
-      | SyntaxKind _ => tt
-      | NativeKind t c => c
-    end.
-
   Fixpoint getCalls {retT} (a: ActionT typeUT retT) (cs: list DefMethT)
   : list DefMethT :=
     match a with
@@ -242,47 +234,4 @@ Section Exts.
   Definition inline (m: Modules) := inlineDms (merge m).
   
 End Exts.
-
-Require Import Semantics.
-
-Section HideExts.
-  Definition hideMeth {A} (l: LabelTP A) (dmn: string) (m: Modules): LabelTP A :=
-    match getAttribute dmn (getDmsBodies m) with
-      | Some dm =>
-        if noCallDm dm dm then
-          match M.find dmn (dms l), M.find dmn (cms l) with
-            | Some v1, Some v2 =>
-              match signIsEq v1 v2 with
-                | left _ => {| ruleMeth := ruleMeth l;
-                               dms := M.remove dmn (dms l);
-                               cms := M.remove dmn (cms l) |}
-                | _ => l
-              end
-            | _, _ => l
-          end
-        else l
-      | _ => l
-    end.
-
-  Fixpoint hideMeths {A} (l: LabelTP A) (dms: list string) (m: Modules): LabelTP A :=
-    match dms with
-      | nil => l
-      | dm :: dms' => hideMeths (hideMeth l dm m) dms' (inlineDmToMod m dm)
-    end.
-
-  Lemma hideMeth_preserves_hide:
-    forall {A} (l: LabelTP A) dm m,
-      hide (hideMeth l dm m) = hide l.
-  Proof.
-    intros; destruct l as [rm dms cms].
-    unfold hide, hideMeth; simpl.
-    destruct (getAttribute dm (getDmsBodies m)); [|reflexivity].
-    destruct (noCallDm a a); [|reflexivity].
-    remember (M.find dm dms) as odm; destruct odm; [|reflexivity].
-    remember (M.find dm cms) as ocm; destruct ocm; [|reflexivity].
-    destruct (signIsEq t t0); [|reflexivity].
-    subst; f_equal; auto; apply M.subtractKV_remove; rewrite <-Heqodm, <-Heqocm; auto.
-  Qed.
-
-End HideExts.
 
